Risc0/Cirgen/Get.lean
@@ -1,0 +1,61 @@
+import Risc0.State
+
+namespace Risc0
+
+  def isGetValid (st : State) (buf : BufferVar) (back : Back) (offset : ℕ) :=
+    back ≤ st.cycle ∧
+    buf ∈ st.vars ∧
+    offset < st.bufferWidths[buf].get! ∧
+    (Buffer.back st buf back offset).isSome
+
+  lemma isGetValid_def :
+    isGetValid st buf back offset = 
+    (back ≤ st.cycle ∧
+    buf ∈ st.vars ∧
+    offset < st.bufferWidths[buf].get! ∧
+    (Buffer.back st buf back offset).isSome) := rfl
+
+  instance : Decidable (isGetValid st buf back offset) := by unfold isGetValid; exact inferInstance
+
+  def getImpl (st : State) (buf : BufferVar) (back : Back) (offset : ℕ) :=
+    if isGetValid st buf back offset
+    then Option.some <| Lit.Val (Buffer.back st buf back offset).get!
+    else .none
+
+  lemma getImpl_def : getImpl st buf back offset = 
+                      if isGetValid st buf back offset
+                      then Option.some <| Lit.Val (Buffer.back st buf back offset).get!
+                      else .none := rfl
+
+  --Review: should any of these be simps?
+  lemma getImpl_none_or_val : getImpl st buf back offset = .none ∨ ∃ x, getImpl st buf back offset = some (.Val x) := by
+    simp [getImpl]
+    aesop
+
+  lemma getImpl_val_of_some : getImpl st buf back offset = some lit → ∃ x, lit = .Val x := by
+    have h: getImpl st buf back offset = .none ∨ ∃ x, getImpl st buf back offset = some (.Val x) := getImpl_none_or_val
+    aesop
+
+  lemma getImpl_skip_none_update : getImpl (st[name] ←ₛ .none) buf back offset = getImpl st buf back offset := by
+    simp [State.update, getImpl, isGetValid, Buffer.back]
+
+  lemma getImpl_skip_val_update : getImpl (st[name] ←ₛ .some (.Val x)) buf back offset = getImpl st buf back offset := by
+    simp [State.update, getImpl, isGetValid, Buffer.back]
+
+  @[simp]
+  lemma getImpl_skip_get_update:
+    getImpl (st[name] ←ₛ getImpl st' buf' back' offset') buf back offset =
+    getImpl st buf back offset := by
+    generalize eq: getImpl st' buf' back' offset' = x
+    cases x with
+    | none => exact getImpl_skip_none_update
+    | some lit =>
+      have h: ∃ x, lit = Lit.Val x := getImpl_val_of_some eq
+      aesop
+
+  lemma getImpl_skip_set_offset (h: offset ≠ offset'):
+    getImpl (State.set! st buf offset val) buf back offset' =
+    getImpl st buf back offset' := by
+      sorry
+
+end Risc0
