Risc0/Cirgen/Op.lean
@@ -1,7 +1,58 @@
-import Risc0.Cirgen.BasicTypes
+import Risc0.Cirgen.Notation
 
-namespace Risc0
+namespace Risc0.Op
 
-  
+open MLIRNotation
 
-end Risc0
+@[simp]
+lemma eval_const : Γ st ⟦@Const α x⟧ₑ = .some (.Val x) := rfl
+
+@[simp]
+lemma eval_true : Γ st ⟦@Op.True α⟧ₑ = .some (.Constraint (_root_.True)) := rfl
+
+@[simp]
+lemma eval_getBuffer : Γ st ⟦@Get α buf back offset⟧ₑ =
+  let val := (st.buffers[buf].get!).get! ((st.cycle - back.toNat), offset)
+  if back ≤ st.cycle ∧ buf ∈ st.vars ∧ offset < st.bufferWidths[buf].get! ∧ val.isSome
+  then .some (.Val val.get!)
+  else .none := rfl
+
+@[simp]
+lemma eval_add : Γ st ⟦@Add α x y⟧ₑ = .some (.Val ((st.felts x).get! + (st.felts y).get!)) := rfl
+
+@[simp]
+lemma eval_sub : Γ st ⟦@Sub α x y⟧ₑ = .some (.Val ((st.felts x).get! - (st.felts y).get!)) := rfl
+
+@[simp]
+lemma eval_mul : Γ st ⟦@Mul α x y⟧ₑ = .some (.Val ((st.felts x).get! * (st.felts y).get!)) := rfl
+
+@[simp]
+lemma eval_isz : Γ st ⟦??₀x⟧ₑ = .some (.Val (if (st.felts x).get! = 0 then 1 else 0)) := rfl
+
+@[simp]
+lemma eval_inv : Γ st ⟦Inv x⟧ₑ = .some (.Val (if st.felts[x].get! = 0 then 0 else st.felts[x].get!⁻¹)) := rfl
+
+@[simp]
+lemma eval_andEqz : Γ st ⟦@AndEqz α c x⟧ₑ =
+                    .some (.Constraint ((st.props c).get! ∧ (st.felts x).get! = 0)) := rfl
+
+@[simp]
+lemma eval_bitAnd :
+  Γ st ⟦@BitAnd α x y⟧ₑ =
+    (.some <| .Val <| feltBitAnd (st.felts x).get! (st.felts y).get!) := rfl
+
+@[simp]
+lemma eval_neg : Γ st ⟦@Neg α x⟧ₑ = .some (.Val (0 - (st.felts x).get!)) := rfl
+
+@[simp]
+lemma eval_pow : Γ st ⟦@Pow α x n⟧ₑ = .some (.Val ((st.felts x).get! ^ n)) := rfl
+
+@[simp]
+lemma eval_andCond :
+  Γ st ⟦@AndCond α old cnd inner⟧ₑ =
+    .some (.Constraint ((st.props old).get! ∧
+                       if (st.felts cnd).get! = 0
+                       then _root_.True
+                       else (st.props inner).get!)) := rfl
+
+end Risc0.Op
