Risc0/State/BufferBack.lean
@@ -1,0 +1,10 @@
+import Risc0.State.Defs
+
+namespace Risc0
+
+  lemma Buffer.back_def {st : State} {buf : BufferVar} {back : Back} :
+    Buffer.back st buf back offset = st.buffers[buf].get!.get! (st.cycle - back.toNat, offset) := rfl
+
+  lemma Buffer.back_zero : Buffer.back st buf 0 k = st.buffers[buf].get!.get! (st.cycle, k) := rfl
+
+end Risc0
