Risc0/State/Set.lean
@@ -1,0 +1,11 @@
+import Risc0.State.Defs
+
+namespace Risc0.State
+
+@[simp]
+lemma set!_felts {st : State} {bufferVar : BufferVar} {offset : ℕ} {val : Felt} :
+  (st.set! bufferVar offset val).felts = st.felts := by
+  unfold set! setBufferElementImpl
+  aesop
+
+end Risc0.State
